Suppose that for some $m_{ji}^\star > 0$, $\lambda_{ij}^{\chi} = 0$. Then $\tilde{\bm{\tau}}_i^\star(\bm{m}_j^\star; \bm{m}_{-j}) = \tilde{\bm{\tau}}_i^\star(\bm{m}_j^\prime; \bm{m}_{-j})$ with $m_{ji}^\prime = 0$, $m_{j, -i}^\prime = m_{j, -i}^\star$. Then,
$$
G_i \left(\tilde{\bm{\tau}}^\star(\bm{m}_i^\prime; \bm{m}_{-i}) \right) - \sum_{j \neq i} m_{ij}^\prime \epsilon^m > G_i \left(\tilde{\bm{\tau}}^\star(\bm{m}_i^\star; \bm{m}_{-i}) \right) - \sum_{j \neq i} m_{ij}^\star \epsilon^m
$$
contradicting the premise that $\bm{m}_j^\star$ is a best response.